add: list_in_list_x64_decode_prop

theory/x64Disassembler.thy
@@ -10,6 +10,457 @@ value "[(1::nat)]!(0::nat)"
 
 value "[(1::nat)]!(1::nat)" returns an error, we should have a nth_error? *)
 
+definition x64_decode_op_0x66 :: "nat \<Rightarrow> x64_bin \<Rightarrow> (nat * instruction) option" where
+"x64_decode_op_0x66 pc l_bin = (
+  case nth_error l_bin (pc+1) of None \<Rightarrow> None | Some h1 \<Rightarrow>
+    if unsigned_bitfield_extract_u8 4 4 h1 \<noteq> 0b0100 then  
+      \<comment> \<open> R7.1 [legacy + opcode + modrm + imm] \<close>
+      case nth_error l_bin (pc+2) of None \<Rightarrow> None | Some reg \<Rightarrow>
+      let modrm = unsigned_bitfield_extract_u8 6 2 reg in
+      let reg1  = unsigned_bitfield_extract_u8 3 3 reg in
+      let reg2  = unsigned_bitfield_extract_u8 0 3 reg in
+      let src   = bitfield_insert_u8 3 1 reg1 0 in
+      let dst   = bitfield_insert_u8 3 1 reg2 0 in
+        if h1 = 0xc1 then 
+       \<comment> \<open> P2887 `ROL : register by immediate count` -> `0x66 1100 000w : 11 000 reg : imm8` \<close>
+          case nth_error l_bin (pc+3) of None \<Rightarrow> None | Some imm \<Rightarrow>
+            if modrm = 0b11 \<and> src = 0b000 then
+              case ireg_of_u8 dst of None \<Rightarrow> None | Some dst \<Rightarrow> (
+                Some (4, Prolw_ri dst imm))
+            else None
+      else if h1 = 0x81 then
+        if modrm = 0b11 then
+          case ireg_of_u8 dst of None \<Rightarrow> None | Some dst \<Rightarrow> (
+            case nth_error l_bin (pc+3) of None \<Rightarrow> None | Some i1 \<Rightarrow> (
+            case nth_error l_bin (pc+4) of None \<Rightarrow> None | Some i2 \<Rightarrow> (
+              case u16_of_u8_list [i1,i2] of None \<Rightarrow> None |
+                Some imm \<Rightarrow> 
+                  \<comment> \<open> P2876 `ADD imm16 to reg16` -> ` 0x66 1000 00sw : 11 000 reg : imm16` \<close>
+                  if reg1 = 0b000 then
+                    Some (5, Paddw_ri dst imm)
+                  else None) ))
+        else None
+      \<comment> \<open> R7.2 [legacy + opcode + modrm + displacement] \<close>
+        else if h1 = 0x89 then 
+          \<comment> \<open> P2882 ` MOV: reg to memory`  ->  `66H 0100 0RXB : 1000 1001 : mod reg r/m `\<close>
+            if modrm = 0b01  then
+              case nth_error l_bin (pc+3) of None \<Rightarrow> None | Some dis \<Rightarrow> ( \<comment> \<open> displacement8 \<close> 
+                case ireg_of_u8 src of None \<Rightarrow> None | Some src \<Rightarrow> (
+                case ireg_of_u8 dst of None \<Rightarrow> None | Some dst \<Rightarrow> ( 
+                    Some (4, Pmov_mr (Addrmode (Some dst) None (scast dis)) src  M16))))
+            else None
+        else None
+    else  
+      let w = unsigned_bitfield_extract_u8 3 1 h1 in
+      let r = unsigned_bitfield_extract_u8 2 1 h1 in
+      let x = unsigned_bitfield_extract_u8 1 1 h1 in
+      let b = unsigned_bitfield_extract_u8 0 1 h1 in (
+        case nth_error l_bin (pc+2) of None \<Rightarrow> None | Some op \<Rightarrow> (
+        case nth_error l_bin (pc+3) of None \<Rightarrow> None | Some reg \<Rightarrow> (
+        let modrm = unsigned_bitfield_extract_u8 6 2 reg in
+        let reg1  = unsigned_bitfield_extract_u8 3 3 reg in
+        let reg2  = unsigned_bitfield_extract_u8 0 3 reg in
+        let src   = bitfield_insert_u8 3 1 reg1 r in
+        let dst   = bitfield_insert_u8 3 1 reg2 b in
+          \<comment> \<open> R7.3 [legacy + rex + opcode + modrm + imm] \<close>
+          if op = 0xc1 then 
+          \<comment> \<open> P2887 `ROL : register by immediate count` -> `0x66 1100 000w : 11 000 reg : imm8` \<close>
+            case nth_error l_bin (pc+4) of None \<Rightarrow> None | Some imm \<Rightarrow> (
+              if modrm = 0b11 \<and> src = 0b000 then
+                case ireg_of_u8 dst of None \<Rightarrow> None | Some dst \<Rightarrow> (
+                  if w = 0 \<and> r = 0 \<and> x = 0 then
+                    Some (5, Prolw_ri dst imm)
+                  else None)
+              else None )
+          else if op = 0x81 then
+            if modrm = 0b11 then
+              case ireg_of_u8 dst of None \<Rightarrow> None | Some dst \<Rightarrow> (
+                case nth_error l_bin (pc+4) of None \<Rightarrow> None | Some i1 \<Rightarrow> (
+                case nth_error l_bin (pc+5) of None \<Rightarrow> None | Some i2 \<Rightarrow> (
+                  case u16_of_u8_list [i1,i2] of None \<Rightarrow> None |
+                    Some imm \<Rightarrow> 
+                      \<comment> \<open> P2876 `ADD imm16 to reg16` -> ` 0x66 1000 00sw : 11 000 reg : imm16` \<close>
+                      if reg1 = 0b000 \<and> w = 0 \<and> r = 0 \<and> x = 0 then
+                        Some (6, Paddw_ri dst imm)
+                      else None) ))
+            else None
+          \<comment> \<open> R7.4 [legacy + rex + opcode + modrm + displacement\<close>
+          else if op = 0x89 then 
+          \<comment> \<open> P2882 ` MOV: reg to memory`  ->  `66H 0100 0RXB : 1000 1001 : mod reg r/m `\<close>
+            if modrm = 0b01  then
+              case nth_error l_bin (pc+4) of None \<Rightarrow> None | Some dis \<Rightarrow> (  \<comment> \<open> displacement8 \<close>
+                  case ireg_of_u8 src of None \<Rightarrow> None | Some src \<Rightarrow> (
+                  case ireg_of_u8 dst of None \<Rightarrow> None | Some dst \<Rightarrow> ( 
+                    if w = 0 \<and> x = 0 then
+                      Some (5, Pmov_mr (Addrmode (Some dst) None (scast dis)) src  M16)
+                    else None )))
+            else None
+          else None )))
+)"
+
+definition x64_decode_op_0x0f :: "nat \<Rightarrow> x64_bin \<Rightarrow> (nat * instruction) option" where
+"x64_decode_op_0x0f pc l_bin = (
+  case nth_error l_bin (pc+1) of None \<Rightarrow> None | Some op \<Rightarrow>
+    \<comment> \<open> R8.1 [escape + opcode] \<close>         
+    if op = 0x31 then 
+      Some (2, Prdtsc)
+    \<comment> \<open> P2877 `BSWAP: register `   -> `0000 1111 : 1100 1 reg` \<close>
+    else if unsigned_bitfield_extract_u8 3 5 op = 0b11001 then
+      let reg2 = unsigned_bitfield_extract_u8 0 3 op in
+      let dst  = bitfield_insert_u8 3 1 reg2 0 in
+        case ireg_of_u8 dst of None \<Rightarrow> None | Some dst \<Rightarrow> (
+          Some (2, Pbswapl dst))
+    \<comment> \<open> R8.2 [escape + opcode + modrm] \<close>
+    \<comment> \<open> P2919 `MOVcc : resgister2  to resgister1 ` -> `0100 0R0B 0000 1111: 0100 tttn : 11 reg1 reg2` \<close>
+    else if unsigned_bitfield_extract_u8 4 4 op = 0b0100 then
+      let flag = (unsigned_bitfield_extract_u8 0 4 op) in 
+      case nth_error l_bin (pc+2) of None \<Rightarrow> None | Some reg \<Rightarrow>
+      let modrm = unsigned_bitfield_extract_u8 6 2 reg in
+      let reg1  = unsigned_bitfield_extract_u8 3 3 reg in
+      let reg2  = unsigned_bitfield_extract_u8 0 3 reg in
+      let src   = bitfield_insert_u8 3 1 reg1 0 in
+      let dst   = bitfield_insert_u8 3 1 reg2 0 in
+        if modrm = 0b11 then
+          case cond_of_u8 flag of None \<Rightarrow> None | Some t \<Rightarrow>(
+          case ireg_of_u8 src of None \<Rightarrow> None | Some src \<Rightarrow> (
+          case ireg_of_u8 dst of None \<Rightarrow> None | Some dst \<Rightarrow> (
+            Some (3, Pcmovl t src dst))))
+        else None
+    \<comment> \<open> R8.3 [escape + opcode + displacement] \<close>
+    \<comment> \<open> P2880 `JCC: full displacement` -> `0000 1111 : 1000 tttn : full displacement` \<close>
+    else if unsigned_bitfield_extract_u8 4 4 op = 0b1000 then
+      let flag = (unsigned_bitfield_extract_u8 0 4 op) in
+      case nth_error l_bin (pc+2) of None \<Rightarrow> None | Some i1 \<Rightarrow> (
+      case nth_error l_bin (pc+3) of None \<Rightarrow> None | Some i2 \<Rightarrow> (
+      case nth_error l_bin (pc+4) of None \<Rightarrow> None | Some i3 \<Rightarrow> (
+      case nth_error l_bin (pc+5) of None \<Rightarrow> None | Some i4 \<Rightarrow> (
+        case u32_of_u8_list [i1,i2,i3,i4] of None \<Rightarrow> None | Some d \<Rightarrow>(
+        case cond_of_u8 flag of None \<Rightarrow> None | Some t \<Rightarrow>(
+          Some(6, Pjcc t d))) ))))
+    else None
+)"
+
+
+definition x64_decode_op_not_rex :: "u8 \<Rightarrow> nat \<Rightarrow> x64_bin \<Rightarrow> (nat * instruction) option" where
+"x64_decode_op_not_rex h pc l_bin = (
+    \<comment> \<open> R1 [opcode] \<close>
+    \<comment> \<open> P2885 `PUSH: qwordregister (alternate encoding)`   -> ` 0100 W00BS : 0101 0 reg64` \<close>
+  if unsigned_bitfield_extract_u8 3 5 h = 0b01010 then
+    let reg2 = unsigned_bitfield_extract_u8 0 3 h in
+    let dst  = bitfield_insert_u8 3 1 reg2 0 in
+    case ireg_of_u8 dst of None \<Rightarrow> None | Some dst \<Rightarrow> (
+    Some (1, Ppushl_r dst))
+    \<comment> \<open> P2885 `POP: qwordregister (alternate encoding)`   -> ` 0100 W00B : 0101 1 reg64 ` \<close>
+    else if unsigned_bitfield_extract_u8 3 5 h = 0b01011 then
+    let reg2 = unsigned_bitfield_extract_u8 0 3 h in
+    let dst  = bitfield_insert_u8 3 1 reg2 0 in
+    case ireg_of_u8 dst of None \<Rightarrow> None | Some dst \<Rightarrow> (
+    Some (1, Ppopl dst))
+    \<comment> \<open> R4 [opcode + displacement] \<close>
+    else if h = 0xe8 then   
+    \<comment> \<open> P2878 `CALL: direct`   -> `1110 1000 : displacement32` \<close>
+    case nth_error l_bin (pc+1) of None \<Rightarrow> None | Some i1 \<Rightarrow> (
+    case nth_error l_bin (pc+2) of None \<Rightarrow> None | Some i2 \<Rightarrow> (
+    case nth_error l_bin (pc+3) of None \<Rightarrow> None | Some i3 \<Rightarrow> (
+    case nth_error l_bin (pc+4) of None \<Rightarrow> None | Some i4 \<Rightarrow> (
+    case u32_of_u8_list [i1,i2,i3,i4] of None \<Rightarrow> None |
+      Some d \<Rightarrow> ( Some (5, Pcall_i (scast d))) ))))
+    else if h = 0xe9 then
+    \<comment> \<open> P2881 `JMP: direct` -> `1110 1001 : displacement32` \<close>
+    case nth_error l_bin (pc+1) of None \<Rightarrow> None | Some i1 \<Rightarrow> (
+    case nth_error l_bin (pc+2) of None \<Rightarrow> None | Some i2 \<Rightarrow> (
+    case nth_error l_bin (pc+3) of None \<Rightarrow> None | Some i3 \<Rightarrow> (
+    case nth_error l_bin (pc+4) of None \<Rightarrow> None | Some i4 \<Rightarrow> (
+    case u32_of_u8_list [i1,i2,i3,i4] of None \<Rightarrow> None |
+      Some d \<Rightarrow> ( Some (5, Pjmp (scast d))) ))))
+    else
+    case nth_error l_bin (pc+1) of None \<Rightarrow> None | Some reg \<Rightarrow>
+    let modrm = unsigned_bitfield_extract_u8 6 2 reg in
+    let reg1  = unsigned_bitfield_extract_u8 3 3 reg in
+    let reg2  = unsigned_bitfield_extract_u8 0 3 reg in
+    let src   = bitfield_insert_u8 3 1 reg1 0 in
+    let dst   = bitfield_insert_u8 3 1 reg2 0 in
+    \<comment> \<open> R2 [opcode + modrm] \<close>
+    if h = 0x89 then 
+    \<comment> \<open> P2887 `MOV register1 to register2` -> `0100 0R0B : 1000 1001 : 11 reg1 reg2` \<close>
+      if modrm = 0b11 then
+        case ireg_of_u8 src of None \<Rightarrow> None | Some src \<Rightarrow> (
+        case ireg_of_u8 dst of None \<Rightarrow> None | Some dst \<Rightarrow> (
+          Some (2, Pmovl_rr dst src)))
+      else if modrm = 0b01 then
+        \<comment> \<open> P2882 ` MOV: reg to memory` ->  `0100 WRXB : 1000 1001 : mod reg r/m` \<close>
+        \<comment> \<open> P2882 ` MOV: qwordregister to memory64` ->  `0100 1RXB 1000 1001 : mod qwordreg r/m` \<close>
+        case nth_error l_bin (pc+2) of None \<Rightarrow> None | Some dis \<Rightarrow> ( \<comment> \<open> displacement8 \<close>
+          case ireg_of_u8 src of None \<Rightarrow> None | Some src \<Rightarrow> (
+          case ireg_of_u8 dst of None \<Rightarrow> None | Some dst \<Rightarrow> ( 
+              Some (3, Pmov_mr (Addrmode (Some dst) None (scast dis)) src M32))))
+      else if modrm = 0b10 then 
+        case nth_error l_bin (pc+2) of None \<Rightarrow> None | Some d1 \<Rightarrow> (
+        case nth_error l_bin (pc+3) of None \<Rightarrow> None | Some d2 \<Rightarrow> (
+        case nth_error l_bin (pc+4) of None \<Rightarrow> None | Some d3 \<Rightarrow> (
+        case nth_error l_bin (pc+5) of None \<Rightarrow> None | Some d4 \<Rightarrow> (
+          case u32_of_u8_list [d1,d2,d3,d4] of None \<Rightarrow> None | Some dis \<Rightarrow>(
+          case ireg_of_u8 src of None \<Rightarrow> None | Some src \<Rightarrow> (
+          case ireg_of_u8 dst of None \<Rightarrow> None | Some dst \<Rightarrow> (
+             Some (6, Pmov_mr (Addrmode (Some dst) None dis) src M32)))) ))))
+      else None
+    else if h = 0x01 then
+    \<comment> \<open> P2876 `ADD register1 to register2` -> `0100 0R0B : 0000 000w : 11 reg1 reg2` \<close>
+      if modrm = 0b11 then
+        case ireg_of_u8 src of None \<Rightarrow> None | Some src \<Rightarrow> (
+        case ireg_of_u8 dst of None \<Rightarrow> None | Some dst \<Rightarrow> (
+          Some (2, Paddl_rr dst src))) 
+      else None
+    \<comment> \<open> P2884 `NEG  register2`   -> `0100 100B : 1111 0111 : 11011reg` \<close>
+    else if h = 0xf7 then
+      if modrm = 0b11 \<and> reg1 = 0b011 then 
+        case ireg_of_u8 dst of None \<Rightarrow> None | Some dst \<Rightarrow> (
+          Some (2, Pnegl dst))
+    \<comment> \<open> P2884 `MUL  AL, AX, or EAX with register2` -> ` 0100 000B : 1111 011w : 11 100 reg` \<close>
+      else if modrm = 0b11 \<and> reg1 = 0b100 then
+        case ireg_of_u8 dst of None \<Rightarrow> None | Some dst \<Rightarrow> (
+          Some (2, Pmull_r dst))
+    \<comment> \<open> P2880 `IMUL AL, AX, or EAX with register2` -> ` 0100 000B : 1111 011w : 11 101 reg` \<close>
+      else if modrm = 0b11 \<and> reg1 = 0b101 then
+        case ireg_of_u8 dst of None \<Rightarrow> None | Some dst \<Rightarrow> (
+           Some (2, Pimull_r dst))
+      else if modrm = 0b11 \<and> reg1 = 0b110 then
+    \<comment> \<open> P2879 `DIV  AL, AX, or EAX by register2`   -> ` 0100 000B : 1111 011w : 11 110 reg` \<close>
+        case ireg_of_u8 dst of None \<Rightarrow> None | Some dst \<Rightarrow> (
+           Some (2, Pdivl_r dst))
+      else if modrm = 0b11 \<and> reg1 = 0b111 then
+    \<comment> \<open> P2879 `IDIV AL, AX, or EAX by register2`   -> ` 0100 000B : 1111 011w : 11 111 reg` \<close>
+        case ireg_of_u8 dst of None \<Rightarrow> None | Some dst \<Rightarrow> (
+           Some (2, Pidivl_r dst))
+     \<comment> \<open> P2892 `TEST: immediate and register`   -> `  1111 011w : 11 000 reg : imm ` \<close>
+      else if modrm = 0b11 \<and> reg1 = 0b000 then
+        case nth_error l_bin (pc+2) of None \<Rightarrow> None | Some i1 \<Rightarrow> (
+        case nth_error l_bin (pc+3) of None \<Rightarrow> None | Some i2 \<Rightarrow> (
+        case nth_error l_bin (pc+4) of None \<Rightarrow> None | Some i3 \<Rightarrow> (
+        case nth_error l_bin (pc+5) of None \<Rightarrow> None | Some i4 \<Rightarrow> (
+          case ireg_of_u8 dst of None \<Rightarrow> None | Some dst \<Rightarrow> (
+              case u32_of_u8_list [i1, i2, i3,i4] of None \<Rightarrow> None |
+                Some imm \<Rightarrow> 
+                    Some (6, Ptestl_ri dst imm)) ))))
+      else None
+    \<comment> \<open> P2891 `SUB register1 from register2` -> `0100 WR0B : 0010 100w : 11 reg1 reg2` \<close> 
+    else if h = 0x29 then
+      if modrm = 0b11 then (
+        case ireg_of_u8 src of None \<Rightarrow> None | Some src \<Rightarrow> (
+        case ireg_of_u8 dst of None \<Rightarrow> None | Some dst \<Rightarrow> (
+          Some (2, Psubl_rr dst src) )))
+      else None
+    \<comment> \<open> P2876 `AND register1 to register2` -> ` 0010 000w : 11 reg1 reg2 ` \<close>
+    else if h = 0x21 then
+      if modrm = 0b11 then (
+        case ireg_of_u8 src of None \<Rightarrow> None | Some src \<Rightarrow> (
+        case ireg_of_u8 dst of None \<Rightarrow> None | Some dst \<Rightarrow> (
+           Some (2, Pandl_rr dst src))) ) 
+      else None
+    \<comment> \<open> P2884 `OR register1 to register2` -> ` 0000 100w : 11 reg1 reg2` \<close>
+    else if h = 0x09 then
+      if modrm = 0b11 then (
+        case ireg_of_u8 src of None \<Rightarrow> None | Some src \<Rightarrow> (
+        case ireg_of_u8 dst of None \<Rightarrow> None | Some dst \<Rightarrow> (
+          Some (2, Porl_rr dst src) )))
+      else None
+    \<comment> \<open> P2893 `XOR register1 to register2` -> ` 0011 000w : 11 reg1 reg2` \<close>
+    else if h = 0x31 then
+      if modrm = 0b11 then (
+        case ireg_of_u8 src of None \<Rightarrow> None | Some src \<Rightarrow> (
+        case ireg_of_u8 dst of None \<Rightarrow> None | Some dst \<Rightarrow> (
+          Some (2, Pxorl_rr dst src))) ) 
+      else None
+    else if h = 0xd3 then
+      \<comment> \<open> P2889 `SHL register by CL`              -> ` 1100 000w : 11 100 reg ` \<close>
+      if modrm = 0b11 \<and> reg1 = 0b100 then 
+        case ireg_of_u8 dst of None \<Rightarrow> None | Some dst \<Rightarrow> (
+          Some (2, Pshll_r dst))
+      \<comment> \<open> P2890 `SHR register by CL`              -> ` 1100 000w : 11 101 reg ` \<close>
+      else if modrm = 0b11 \<and> reg1 = 0b101 then
+        case ireg_of_u8 dst of None \<Rightarrow> None | Some dst \<Rightarrow> (
+          Some (2, Pshrl_r dst))  
+      \<comment> \<open> P2888 `SAR register by CL`              -> ` 1100 000w : 11 111 reg ` \<close>
+      else if modrm = 0b11 \<and> reg1 = 0b111 then
+        case ireg_of_u8 dst of None \<Rightarrow> None | Some dst \<Rightarrow> (
+          Some (2, Psarl_r dst))  
+    else None
+    \<comment> \<open> P2892 `TEST: register1 and register2`   -> ` 1000 010w : 11 reg1 reg2` \<close>
+    else if h = 0x85 then
+      if modrm = 0b11 then(
+        case ireg_of_u8 src of None \<Rightarrow> None | Some src \<Rightarrow> (
+        case ireg_of_u8 dst of None \<Rightarrow> None | Some dst \<Rightarrow> (
+          Some(2, Ptestl_rr dst src) )))
+      else None
+    \<comment> \<open> P2878 `CMP: register1 with register2`   -> ` 0011 100w : 11 reg1 reg2 ` \<close>
+    else if h = 0x39 then
+      if modrm = 0b11 then(
+        case ireg_of_u8 src of None \<Rightarrow> None | Some src \<Rightarrow> (
+        case ireg_of_u8 dst of None \<Rightarrow> None | Some dst \<Rightarrow> (
+          Some(2, Pcmpl_rr src dst) )))
+      else None
+    else if h = 0xff then
+    \<comment> \<open> P2878 `CALL: register indirect`   -> `0100 W00Bw 1111 1111 : 11 010 reg ` \<close>
+      if modrm = 0b11 \<and> reg1 = 0b010 then
+        case ireg_of_u8 dst of None \<Rightarrow> None | Some dst \<Rightarrow> (
+          Some (2, Pcall_r dst)) 
+      else None
+    \<comment> \<open> R3 [opcode + modrm + imm] \<close>
+    \<comment> \<open> P2882 `MOV immediate to register` -> ` 1100 011w : 11 000 reg : imm` \<close>
+    else if h = 0xc7 then
+      case nth_error l_bin (pc+2) of None \<Rightarrow> None | Some i1 \<Rightarrow> (
+      case nth_error l_bin (pc+3) of None \<Rightarrow> None | Some i2 \<Rightarrow> (
+      case nth_error l_bin (pc+4) of None \<Rightarrow> None | Some i3 \<Rightarrow> (
+      case nth_error l_bin (pc+5) of None \<Rightarrow> None | Some i4 \<Rightarrow> (
+      case ireg_of_u8 dst of None \<Rightarrow> None | Some dst \<Rightarrow> (
+      case u32_of_u8_list [i1, i2, i3, i4] of None \<Rightarrow> None |
+          Some imm \<Rightarrow> 
+            if modrm = 0b11 \<and> reg1 = 0b000 then
+              Some (6, Pmovl_ri dst imm)
+            else None) ))))
+    else if h = 0xc1 then
+      case nth_error l_bin (pc+2) of None \<Rightarrow> None | Some imm \<Rightarrow> ( 
+        \<comment> \<open> P2889 `SHL register by immediate count`      -> `1100 000w : 11 100 reg : imm8 ` \<close>
+        if modrm = 0b11 \<and> reg1 = 0b100 then 
+          case ireg_of_u8 dst of None \<Rightarrow> None | Some dst \<Rightarrow> (
+             Some (3, Pshll_ri dst imm))
+        \<comment> \<open> P2890 `SHR register by immediate count`      -> ` 1100 000w : 11 101 reg : imm8 ` \<close>
+        else if modrm = 0b11 \<and> reg1 = 0b101 then 
+          case ireg_of_u8 dst of None \<Rightarrow> None | Some dst \<Rightarrow> (
+             Some (3, Pshrl_ri dst imm))
+        \<comment> \<open> P2888 `SAR register by immediate count`      -> `1100 000w : 11 111 reg : imm8 ` \<close>
+        else if modrm = 0b11 \<and> reg1 = 0b111 then 
+          case ireg_of_u8 dst of None \<Rightarrow> None | Some dst \<Rightarrow> (
+             Some (3, Psarl_ri dst imm))
+         else None)
+    else if h = 0x81 then
+      if modrm = 0b11 then
+        case ireg_of_u8 dst of None \<Rightarrow> None | Some dst \<Rightarrow> (
+          case nth_error l_bin (pc+2) of None \<Rightarrow> None | Some i1 \<Rightarrow> (
+          case nth_error l_bin (pc+3) of None \<Rightarrow> None | Some i2 \<Rightarrow> (
+          case nth_error l_bin (pc+4) of None \<Rightarrow> None | Some i3 \<Rightarrow> (
+          case nth_error l_bin (pc+5) of None \<Rightarrow> None | Some i4 \<Rightarrow> (
+            case u32_of_u8_list [i1,i2,i3,i4] of None \<Rightarrow> None |
+              Some imm \<Rightarrow> 
+                \<comment> \<open> P2876 `ADD immediate to register` -> ` 1000 00sw : 11 000 reg : immediate data` \<close>
+                if reg1 = 0b000 then
+                  Some (6, Paddl_ri dst imm)
+                \<comment> \<open> P2891 `OR: immediate to register` -> `0100 000B  1000 00sw : 11 001 reg : imm` \<close>
+                else if reg1 = 0b001 then
+                  Some (6, Porl_ri dst imm)
+                \<comment> \<open> P2891 `AND: immediate to register` -> `0100 000B : 1000 00sw : 11 100 reg : immediate` \<close>
+                else if reg1 = 0b100 then
+                  Some (6, Pandl_ri dst imm)
+                \<comment> \<open> P2891 `SUB: immediate from register` -> `0100 000B 1000 00sw : 11 101 reg : imm` \<close>
+                else if reg1 = 0b101 then
+                  Some (6, Psubl_ri dst imm)
+                \<comment> \<open> P2893 `XOR: immediate to register` -> ` 0100 000B 1000 00sw : 11 110 reg : imm` \<close>
+                else if reg1 = 0b110 then
+                  Some (6, Pxorl_ri dst imm)
+                \<comment> \<open> P2878 `CMP: immediate32 with qwordregister`   -> `0100 100B 1000 0001 : 11 111 qwordreg : imm32` \<close>
+                else if reg1 = 0b111 then
+                  Some (6, Pcmpl_ri dst imm)
+                else None) ))))
+      else None
+    \<comment> \<open> R5 [opcode + modrm + displacement] \<close>
+    \<comment> \<open> P2882 ` MOV: memory to reg`   ->  `0100 0RXB : 1000 101w : mod reg r/m`\<close>
+    else if h = 0x88 then
+      if modrm = 0b01  then
+        case nth_error l_bin (pc+2) of None \<Rightarrow> None | Some dis \<Rightarrow> ( \<comment> \<open> displacement8 \<close>
+          case ireg_of_u8 src of None \<Rightarrow> None | Some src \<Rightarrow> (
+          case ireg_of_u8 dst of None \<Rightarrow> None | Some dst \<Rightarrow> ( 
+            Some (3, Pmov_mr (Addrmode (Some dst) None (scast dis)) src  M8))) )
+      else None
+    else if h = 0x8b then 
+      if modrm = 0b01 then
+        case nth_error l_bin (pc+2) of None \<Rightarrow> None | Some dis \<Rightarrow> ( \<comment> \<open> displacement8 \<close>
+            case ireg_of_u8 src of None \<Rightarrow> None | Some src \<Rightarrow> (
+            case ireg_of_u8 dst of None \<Rightarrow> None | Some dst \<Rightarrow> (
+              Some (3, Pmov_rm src (Addrmode (Some dst) None (scast dis))  M32))) )
+      else if modrm = 0b10 then \<comment> \<open> displacement32 \<close>
+        case nth_error l_bin (pc+2) of None \<Rightarrow> None | Some d1 \<Rightarrow> (
+        case nth_error l_bin (pc+3) of None \<Rightarrow> None | Some d2 \<Rightarrow> (
+        case nth_error l_bin (pc+4) of None \<Rightarrow> None | Some d3 \<Rightarrow> (
+        case nth_error l_bin (pc+5) of None \<Rightarrow> None | Some d4 \<Rightarrow> (
+          case u32_of_u8_list [d1,d2,d3,d4] of None \<Rightarrow> None | Some dis \<Rightarrow>(
+          case ireg_of_u8 src of None \<Rightarrow> None | Some src \<Rightarrow> (
+          case ireg_of_u8 dst of None \<Rightarrow> None | Some dst \<Rightarrow> (
+             Some (6, Pmov_rm src (Addrmode (Some dst) None dis) M32)))) ))))
+      else None
+    else None
+)"
+
+definition x64_decode_op_0x81 :: "u8 \<Rightarrow> u8 \<Rightarrow> u8 \<Rightarrow> u8 \<Rightarrow> u8 \<Rightarrow> u8 \<Rightarrow> u8 \<Rightarrow> u8 \<Rightarrow> nat \<Rightarrow> x64_bin \<Rightarrow> (nat * instruction) option" where
+"x64_decode_op_0x81 modrm dst reg1 reg2 w r x b pc l_bin = (
+  if modrm = 0b11 then
+    case ireg_of_u8 dst of None \<Rightarrow> None | Some dst \<Rightarrow> (
+    case nth_error l_bin (pc+3) of None \<Rightarrow> None | Some i1 \<Rightarrow> (
+    case nth_error l_bin (pc+4) of None \<Rightarrow> None | Some i2 \<Rightarrow> (
+    case nth_error l_bin (pc+5) of None \<Rightarrow> None | Some i3 \<Rightarrow> (
+    case nth_error l_bin (pc+6) of None \<Rightarrow> None | Some i4 \<Rightarrow> (
+      case u32_of_u8_list [i1,i2,i3,i4] of None \<Rightarrow> None |
+        Some imm \<Rightarrow> (
+          \<comment> \<open> P2876 `ADD immediate to register` -> `0100 000B : 1000 00sw : 11 000 reg : immediate data` \<close>
+          if reg1 = 0b000 then
+            if w = 0 \<and> r = 0 \<and> x = 0 then
+              Some (7, Paddl_ri dst imm)
+            else None
+          \<comment> \<open> P2891 `OR: immediate to register` -> `0100 000B  1000 00sw : 11 001 reg : imm` \<close>
+          else if reg1 = 0b001 then
+            if w = 0 \<and> r = 0 \<and> x = 0 then
+              Some (7, Porl_ri dst imm)
+            else None
+          \<comment> \<open> P2891 `AND: immediate to register` -> `0100 000B : 1000 00sw : 11 100 reg : immediate` \<close>
+          else if reg1 = 0b100 then
+            if w = 0 \<and> r = 0 \<and> x = 0 then
+              Some (7, Pandl_ri dst imm)
+            else None
+          \<comment> \<open> P2891 `SUB: immediate from register` -> `0100 000B 1000 00sw : 11 101 reg : imm` \<close>
+          else if reg1 = 0b101 then
+            if w = 0 \<and> r = 0 \<and> x = 0 then
+              Some (7, Psubl_ri dst imm)
+            else None
+          \<comment> \<open> P2893 `XOR: immediate to register` -> ` 0100 000B 1000 00sw : 11 110 reg : imm` \<close>
+          else if reg1 = 0b110 then
+            if w = 0 \<and> r = 0 \<and> x = 0 then
+              Some (7, Pxorl_ri dst imm)
+            else None
+          \<comment> \<open> P2878 `CMP: immediate with register`   -> `0100 000B 1000 00sw : 11 111 reg : imm` \<close>
+          \<comment> \<open> P2878 `CMP: immediate32 with qwordregister`   -> `0100 100B 1000 0001 : 11 111 qwordreg : imm32` \<close>
+          else if reg1 = 0b111 then
+            if w = 1 \<and> r = 0 \<and> x = 0 then
+              Some (7, Pcmpq_ri dst imm)
+            else if w = 0 \<and> r = 0 \<and> x = 0 then
+              Some (7, Pcmpl_ri dst imm)
+            else None
+          else None)) ))))
+  else if modrm = 0b10 \<and> reg2 = 0b100 then
+    case nth_error l_bin (pc+3) of None \<Rightarrow> None | Some sib \<Rightarrow> (
+    let rbase  = unsigned_bitfield_extract_u8 0 3 sib in
+    let rindex = unsigned_bitfield_extract_u8 3 3 sib in
+    let scale  = unsigned_bitfield_extract_u8 6 2 sib in
+    let index  = bitfield_insert_u8 3 1 rindex x in
+    let base   = bitfield_insert_u8 3 1 rbase  b in
+      case nth_error l_bin (pc+4) of None \<Rightarrow> None | Some d1 \<Rightarrow> (
+      case nth_error l_bin (pc+5) of None \<Rightarrow> None | Some d2 \<Rightarrow> (
+      case nth_error l_bin (pc+6) of None \<Rightarrow> None | Some d3 \<Rightarrow> (
+      case nth_error l_bin (pc+7) of None \<Rightarrow> None | Some d4 \<Rightarrow> (
+        case u32_of_u8_list [d1,d2,d3,d4] of None \<Rightarrow> None | Some dis \<Rightarrow>(
+        if reg1 = 0b000 then
+          case nth_error l_bin (pc+8) of None \<Rightarrow> None | Some i1 \<Rightarrow> (
+          case nth_error l_bin (pc+9) of None \<Rightarrow> None | Some i2 \<Rightarrow> (
+          case nth_error l_bin (pc+10) of None \<Rightarrow> None | Some i3 \<Rightarrow> (
+          case nth_error l_bin (pc+11) of None \<Rightarrow> None | Some i4 \<Rightarrow> (
+          case u32_of_u8_list [i1,i2,i3,i4] of None \<Rightarrow> None | Some imm \<Rightarrow> (
+          if w = 1 \<and> r = 0 then
+            case ireg_of_u8 index of None \<Rightarrow> None | Some ri \<Rightarrow> (
+            case ireg_of_u8 base  of None \<Rightarrow> None | Some rb \<Rightarrow> (
+              Some (12, Paddq_mi (Addrmode (Some rb) (Some (ri, scale)) (scast dis)) imm M64 )))
+          else None) ))))
+        else None) )))) )
+  else None
+)"
+
 definition x64_decode :: "nat \<Rightarrow> x64_bin \<Rightarrow> (nat * instruction) option" where
 "x64_decode pc l_bin = (
   case nth_error l_bin pc of None \<Rightarrow> None | Some h \<Rightarrow> \<comment> \<open> R1 [opcode] \<close>
@@ -23,375 +474,11 @@ definition x64_decode :: "nat \<Rightarrow> x64_bin \<Rightarrow> (nat * instruc
       Some (1, Pret)
     \<comment> \<open> R7 legacy \<close>
     else if h = 0x66 then  \<comment> \<open> 16-bit mode \<close>
-      case nth_error l_bin (pc+1) of None \<Rightarrow> None | Some h1 \<Rightarrow>
-        if unsigned_bitfield_extract_u8 4 4 h1 \<noteq> 0b0100 then  
-          \<comment> \<open> R7.1 [legacy + opcode + modrm + imm] \<close>
-          case nth_error l_bin (pc+2) of None \<Rightarrow> None | Some reg \<Rightarrow>
-          let modrm = unsigned_bitfield_extract_u8 6 2 reg in
-          let reg1  = unsigned_bitfield_extract_u8 3 3 reg in
-          let reg2  = unsigned_bitfield_extract_u8 0 3 reg in
-          let src   = bitfield_insert_u8 3 1 reg1 0 in
-          let dst   = bitfield_insert_u8 3 1 reg2 0 in
-            if h1 = 0xc1 then 
-           \<comment> \<open> P2887 `ROL : register by immediate count` -> `0x66 1100 000w : 11 000 reg : imm8` \<close>
-              case nth_error l_bin (pc+3) of None \<Rightarrow> None | Some imm \<Rightarrow>
-                if modrm = 0b11 \<and> src = 0b000 then
-                  case ireg_of_u8 dst of None \<Rightarrow> None | Some dst \<Rightarrow> (
-                    Some (4, Prolw_ri dst imm))
-                else None
-          else if h1 = 0x81 then
-            if modrm = 0b11 then
-              case ireg_of_u8 dst of None \<Rightarrow> None | Some dst \<Rightarrow> (
-                case nth_error l_bin (pc+3) of None \<Rightarrow> None | Some i1 \<Rightarrow> (
-                case nth_error l_bin (pc+4) of None \<Rightarrow> None | Some i2 \<Rightarrow> (
-                  case u16_of_u8_list [i1,i2] of None \<Rightarrow> None |
-                    Some imm \<Rightarrow> 
-                      \<comment> \<open> P2876 `ADD imm16 to reg16` -> ` 0x66 1000 00sw : 11 000 reg : imm16` \<close>
-                      if reg1 = 0b000 then
-                        Some (5, Paddw_ri dst imm)
-                      else None) ))
-            else None
-          \<comment> \<open> R7.2 [legacy + opcode + modrm + displacement] \<close>
-            else if h1 = 0x89 then 
-              \<comment> \<open> P2882 ` MOV: reg to memory`  ->  `66H 0100 0RXB : 1000 1001 : mod reg r/m `\<close>
-                if modrm = 0b01  then
-                  case nth_error l_bin (pc+3) of None \<Rightarrow> None | Some dis \<Rightarrow> ( \<comment> \<open> displacement8 \<close> 
-                    case ireg_of_u8 src of None \<Rightarrow> None | Some src \<Rightarrow> (
-                    case ireg_of_u8 dst of None \<Rightarrow> None | Some dst \<Rightarrow> ( 
-                        Some (4, Pmov_mr (Addrmode (Some dst) None (scast dis)) src  M16))))
-                else None
-            else None
-        else  
-          let w = unsigned_bitfield_extract_u8 3 1 h1 in
-          let r = unsigned_bitfield_extract_u8 2 1 h1 in
-          let x = unsigned_bitfield_extract_u8 1 1 h1 in
-          let b = unsigned_bitfield_extract_u8 0 1 h1 in (
-            case nth_error l_bin (pc+2) of None \<Rightarrow> None | Some op \<Rightarrow> (
-            case nth_error l_bin (pc+3) of None \<Rightarrow> None | Some reg \<Rightarrow> (
-            let modrm = unsigned_bitfield_extract_u8 6 2 reg in
-            let reg1  = unsigned_bitfield_extract_u8 3 3 reg in
-            let reg2  = unsigned_bitfield_extract_u8 0 3 reg in
-            let src   = bitfield_insert_u8 3 1 reg1 r in
-            let dst   = bitfield_insert_u8 3 1 reg2 b in
-              \<comment> \<open> R7.3 [legacy + rex + opcode + modrm + imm] \<close>
-              if op = 0xc1 then 
-              \<comment> \<open> P2887 `ROL : register by immediate count` -> `0x66 1100 000w : 11 000 reg : imm8` \<close>
-                case nth_error l_bin (pc+4) of None \<Rightarrow> None | Some imm \<Rightarrow> (
-                  if modrm = 0b11 \<and> src = 0b000 then
-                    case ireg_of_u8 dst of None \<Rightarrow> None | Some dst \<Rightarrow> (
-                      if w = 0 \<and> r = 0 \<and> x = 0 then
-                        Some (5, Prolw_ri dst imm)
-                      else None)
-                  else None )
-              else if op = 0x81 then
-                if modrm = 0b11 then
-                  case ireg_of_u8 dst of None \<Rightarrow> None | Some dst \<Rightarrow> (
-                    case nth_error l_bin (pc+4) of None \<Rightarrow> None | Some i1 \<Rightarrow> (
-                    case nth_error l_bin (pc+5) of None \<Rightarrow> None | Some i2 \<Rightarrow> (
-                      case u16_of_u8_list [i1,i2] of None \<Rightarrow> None |
-                        Some imm \<Rightarrow> 
-                          \<comment> \<open> P2876 `ADD imm16 to reg16` -> ` 0x66 1000 00sw : 11 000 reg : imm16` \<close>
-                          if reg1 = 0b000 \<and> w = 0 \<and> r = 0 \<and> x = 0 then
-                            Some (6, Paddw_ri dst imm)
-                          else None) ))
-                else None
-              \<comment> \<open> R7.4 [legacy + rex + opcode + modrm + displacement\<close>
-              else if op = 0x89 then 
-              \<comment> \<open> P2882 ` MOV: reg to memory`  ->  `66H 0100 0RXB : 1000 1001 : mod reg r/m `\<close>
-                if modrm = 0b01  then
-                  case nth_error l_bin (pc+4) of None \<Rightarrow> None | Some dis \<Rightarrow> (  \<comment> \<open> displacement8 \<close>
-                      case ireg_of_u8 src of None \<Rightarrow> None | Some src \<Rightarrow> (
-                      case ireg_of_u8 dst of None \<Rightarrow> None | Some dst \<Rightarrow> ( 
-                        if w = 0 \<and> x = 0 then
-                          Some (5, Pmov_mr (Addrmode (Some dst) None (scast dis)) src  M16)
-                        else None )))
-                else None
-              else None )))
+      x64_decode_op_0x66 pc l_bin
     else if h = 0x0f then \<comment> \<open> R8 escape \<close>
-      case nth_error l_bin (pc+1) of None \<Rightarrow> None | Some op \<Rightarrow>
-        \<comment> \<open> R8.1 [escape + opcode] \<close>         
-        if op = 0x31 then 
-          Some (2, Prdtsc)
-        \<comment> \<open> P2877 `BSWAP: register `   -> `0000 1111 : 1100 1 reg` \<close>
-        else if unsigned_bitfield_extract_u8 3 5 op = 0b11001 then
-          let reg2 = unsigned_bitfield_extract_u8 0 3 op in
-          let dst  = bitfield_insert_u8 3 1 reg2 0 in
-            case ireg_of_u8 dst of None \<Rightarrow> None | Some dst \<Rightarrow> (
-              Some (2, Pbswapl dst))
-        \<comment> \<open> R8.2 [escape + opcode + modrm] \<close>
-        \<comment> \<open> P2919 `MOVcc : resgister2  to resgister1 ` -> `0100 0R0B 0000 1111: 0100 tttn : 11 reg1 reg2` \<close>
-        else if unsigned_bitfield_extract_u8 4 4 op = 0b0100 then
-          let flag = (unsigned_bitfield_extract_u8 0 4 op) in 
-          case nth_error l_bin (pc+2) of None \<Rightarrow> None | Some reg \<Rightarrow>
-          let modrm = unsigned_bitfield_extract_u8 6 2 reg in
-          let reg1  = unsigned_bitfield_extract_u8 3 3 reg in
-          let reg2  = unsigned_bitfield_extract_u8 0 3 reg in
-          let src   = bitfield_insert_u8 3 1 reg1 0 in
-          let dst   = bitfield_insert_u8 3 1 reg2 0 in
-            if modrm = 0b11 then
-              case cond_of_u8 flag of None \<Rightarrow> None | Some t \<Rightarrow>(
-              case ireg_of_u8 src of None \<Rightarrow> None | Some src \<Rightarrow> (
-              case ireg_of_u8 dst of None \<Rightarrow> None | Some dst \<Rightarrow> (
-                Some (3, Pcmovl t src dst))))
-            else None
-        \<comment> \<open> R8.3 [escape + opcode + displacement] \<close>
-        \<comment> \<open> P2880 `JCC: full displacement` -> `0000 1111 : 1000 tttn : full displacement` \<close>
-        else if unsigned_bitfield_extract_u8 4 4 op = 0b1000 then
-          let flag = (unsigned_bitfield_extract_u8 0 4 op) in
-          case nth_error l_bin (pc+2) of None \<Rightarrow> None | Some i1 \<Rightarrow> (
-          case nth_error l_bin (pc+3) of None \<Rightarrow> None | Some i2 \<Rightarrow> (
-          case nth_error l_bin (pc+4) of None \<Rightarrow> None | Some i3 \<Rightarrow> (
-          case nth_error l_bin (pc+5) of None \<Rightarrow> None | Some i4 \<Rightarrow> (
-            case u32_of_u8_list [i1,i2,i3,i4] of None \<Rightarrow> None | Some d \<Rightarrow>(
-            case cond_of_u8 flag of None \<Rightarrow> None | Some t \<Rightarrow>(
-              Some(6, Pjcc t d))) ))))
-        else None
+      x64_decode_op_0x0f pc l_bin
     else if unsigned_bitfield_extract_u8 4 4 h \<noteq> 0b0100 then  \<comment> \<open> h is not rex  \<close>
-        \<comment> \<open> R1 [opcode] \<close>
-        \<comment> \<open> P2885 `PUSH: qwordregister (alternate encoding)`   -> ` 0100 W00BS : 0101 0 reg64` \<close>
-        if unsigned_bitfield_extract_u8 3 5 h = 0b01010 then
-          let reg2 = unsigned_bitfield_extract_u8 0 3 h in
-          let dst  = bitfield_insert_u8 3 1 reg2 0 in
-          case ireg_of_u8 dst of None \<Rightarrow> None | Some dst \<Rightarrow> (
-            Some (1, Ppushl_r dst))
-        \<comment> \<open> P2885 `POP: qwordregister (alternate encoding)`   -> ` 0100 W00B : 0101 1 reg64 ` \<close>
-        else if unsigned_bitfield_extract_u8 3 5 h = 0b01011 then
-          let reg2 = unsigned_bitfield_extract_u8 0 3 h in
-          let dst  = bitfield_insert_u8 3 1 reg2 0 in
-          case ireg_of_u8 dst of None \<Rightarrow> None | Some dst \<Rightarrow> (
-            Some (1, Ppopl dst))
-        \<comment> \<open> R4 [opcode + displacement] \<close>
-        else if h = 0xe8 then   
-          \<comment> \<open> P2878 `CALL: direct`   -> `1110 1000 : displacement32` \<close>
-          case nth_error l_bin (pc+1) of None \<Rightarrow> None | Some i1 \<Rightarrow> (
-          case nth_error l_bin (pc+2) of None \<Rightarrow> None | Some i2 \<Rightarrow> (
-          case nth_error l_bin (pc+3) of None \<Rightarrow> None | Some i3 \<Rightarrow> (
-          case nth_error l_bin (pc+4) of None \<Rightarrow> None | Some i4 \<Rightarrow> (
-            case u32_of_u8_list [i1,i2,i3,i4] of None \<Rightarrow> None |
-              Some d \<Rightarrow> ( Some (5, Pcall_i (scast d))) ))))
-        else if h = 0xe9 then
-          \<comment> \<open> P2881 `JMP: direct` -> `1110 1001 : displacement32` \<close>
-          case nth_error l_bin (pc+1) of None \<Rightarrow> None | Some i1 \<Rightarrow> (
-          case nth_error l_bin (pc+2) of None \<Rightarrow> None | Some i2 \<Rightarrow> (
-          case nth_error l_bin (pc+3) of None \<Rightarrow> None | Some i3 \<Rightarrow> (
-          case nth_error l_bin (pc+4) of None \<Rightarrow> None | Some i4 \<Rightarrow> (
-            case u32_of_u8_list [i1,i2,i3,i4] of None \<Rightarrow> None |
-              Some d \<Rightarrow> ( Some (5, Pjmp (scast d))) ))))
-        else
-          case nth_error l_bin (pc+1) of None \<Rightarrow> None | Some reg \<Rightarrow>
-          let modrm = unsigned_bitfield_extract_u8 6 2 reg in
-          let reg1  = unsigned_bitfield_extract_u8 3 3 reg in
-          let reg2  = unsigned_bitfield_extract_u8 0 3 reg in
-          let src   = bitfield_insert_u8 3 1 reg1 0 in
-          let dst   = bitfield_insert_u8 3 1 reg2 0 in
-            \<comment> \<open> R2 [opcode + modrm] \<close>
-            if h = 0x89 then 
-            \<comment> \<open> P2887 `MOV register1 to register2` -> `0100 0R0B : 1000 1001 : 11 reg1 reg2` \<close>
-              if modrm = 0b11 then
-                case ireg_of_u8 src of None \<Rightarrow> None | Some src \<Rightarrow> (
-                case ireg_of_u8 dst of None \<Rightarrow> None | Some dst \<Rightarrow> (
-                  Some (2, Pmovl_rr dst src)))
-              else if modrm = 0b01 then
-                \<comment> \<open> P2882 ` MOV: reg to memory` ->  `0100 WRXB : 1000 1001 : mod reg r/m` \<close>
-                \<comment> \<open> P2882 ` MOV: qwordregister to memory64` ->  `0100 1RXB 1000 1001 : mod qwordreg r/m` \<close>
-                case nth_error l_bin (pc+2) of None \<Rightarrow> None | Some dis \<Rightarrow> ( \<comment> \<open> displacement8 \<close>
-                  case ireg_of_u8 src of None \<Rightarrow> None | Some src \<Rightarrow> (
-                  case ireg_of_u8 dst of None \<Rightarrow> None | Some dst \<Rightarrow> ( 
-                      Some (3, Pmov_mr (Addrmode (Some dst) None (scast dis)) src M32))))
-              else if modrm = 0b10 then 
-                case nth_error l_bin (pc+2) of None \<Rightarrow> None | Some d1 \<Rightarrow> (
-                case nth_error l_bin (pc+3) of None \<Rightarrow> None | Some d2 \<Rightarrow> (
-                case nth_error l_bin (pc+4) of None \<Rightarrow> None | Some d3 \<Rightarrow> (
-                case nth_error l_bin (pc+5) of None \<Rightarrow> None | Some d4 \<Rightarrow> (
-                  case u32_of_u8_list [d1,d2,d3,d4] of None \<Rightarrow> None | Some dis \<Rightarrow>(
-                  case ireg_of_u8 src of None \<Rightarrow> None | Some src \<Rightarrow> (
-                  case ireg_of_u8 dst of None \<Rightarrow> None | Some dst \<Rightarrow> (
-                     Some (6, Pmov_mr (Addrmode (Some dst) None dis) src M32)))) ))))
-              else None
-            else if h = 0x01 then
-            \<comment> \<open> P2876 `ADD register1 to register2` -> `0100 0R0B : 0000 000w : 11 reg1 reg2` \<close>
-              if modrm = 0b11 then
-                case ireg_of_u8 src of None \<Rightarrow> None | Some src \<Rightarrow> (
-                case ireg_of_u8 dst of None \<Rightarrow> None | Some dst \<Rightarrow> (
-                  Some (2, Paddl_rr dst src))) 
-              else None
-            \<comment> \<open> P2884 `NEG  register2`   -> `0100 100B : 1111 0111 : 11011reg` \<close>
-            else if h = 0xf7 then
-              if modrm = 0b11 \<and> reg1 = 0b011 then 
-                case ireg_of_u8 dst of None \<Rightarrow> None | Some dst \<Rightarrow> (
-                  Some (2, Pnegl dst))
-            \<comment> \<open> P2884 `MUL  AL, AX, or EAX with register2` -> ` 0100 000B : 1111 011w : 11 100 reg` \<close>
-              else if modrm = 0b11 \<and> reg1 = 0b100 then
-                case ireg_of_u8 dst of None \<Rightarrow> None | Some dst \<Rightarrow> (
-                  Some (2, Pmull_r dst))
-            \<comment> \<open> P2880 `IMUL AL, AX, or EAX with register2` -> ` 0100 000B : 1111 011w : 11 101 reg` \<close>
-              else if modrm = 0b11 \<and> reg1 = 0b101 then
-                case ireg_of_u8 dst of None \<Rightarrow> None | Some dst \<Rightarrow> (
-                   Some (2, Pimull_r dst))
-              else if modrm = 0b11 \<and> reg1 = 0b110 then
-            \<comment> \<open> P2879 `DIV  AL, AX, or EAX by register2`   -> ` 0100 000B : 1111 011w : 11 110 reg` \<close>
-                case ireg_of_u8 dst of None \<Rightarrow> None | Some dst \<Rightarrow> (
-                   Some (2, Pdivl_r dst))
-              else if modrm = 0b11 \<and> reg1 = 0b111 then
-            \<comment> \<open> P2879 `IDIV AL, AX, or EAX by register2`   -> ` 0100 000B : 1111 011w : 11 111 reg` \<close>
-                case ireg_of_u8 dst of None \<Rightarrow> None | Some dst \<Rightarrow> (
-                   Some (2, Pidivl_r dst))
-             \<comment> \<open> P2892 `TEST: immediate and register`   -> `  1111 011w : 11 000 reg : imm ` \<close>
-              else if modrm = 0b11 \<and> reg1 = 0b000 then
-                case nth_error l_bin (pc+2) of None \<Rightarrow> None | Some i1 \<Rightarrow> (
-                case nth_error l_bin (pc+3) of None \<Rightarrow> None | Some i2 \<Rightarrow> (
-                case nth_error l_bin (pc+4) of None \<Rightarrow> None | Some i3 \<Rightarrow> (
-                case nth_error l_bin (pc+5) of None \<Rightarrow> None | Some i4 \<Rightarrow> (
-                  case ireg_of_u8 dst of None \<Rightarrow> None | Some dst \<Rightarrow> (
-                      case u32_of_u8_list [i1, i2, i3,i4] of None \<Rightarrow> None |
-                        Some imm \<Rightarrow> 
-                            Some (6, Ptestl_ri dst imm)) ))))
-              else None
-            \<comment> \<open> P2891 `SUB register1 from register2` -> `0100 WR0B : 0010 100w : 11 reg1 reg2` \<close> 
-            else if h = 0x29 then
-              if modrm = 0b11 then (
-                case ireg_of_u8 src of None \<Rightarrow> None | Some src \<Rightarrow> (
-                case ireg_of_u8 dst of None \<Rightarrow> None | Some dst \<Rightarrow> (
-                  Some (2, Psubl_rr dst src) )))
-              else None
-            \<comment> \<open> P2876 `AND register1 to register2` -> ` 0010 000w : 11 reg1 reg2 ` \<close>
-            else if h = 0x21 then
-              if modrm = 0b11 then (
-                case ireg_of_u8 src of None \<Rightarrow> None | Some src \<Rightarrow> (
-                case ireg_of_u8 dst of None \<Rightarrow> None | Some dst \<Rightarrow> (
-                   Some (2, Pandl_rr dst src))) ) 
-              else None
-            \<comment> \<open> P2884 `OR register1 to register2` -> ` 0000 100w : 11 reg1 reg2` \<close>
-            else if h = 0x09 then
-              if modrm = 0b11 then (
-                case ireg_of_u8 src of None \<Rightarrow> None | Some src \<Rightarrow> (
-                case ireg_of_u8 dst of None \<Rightarrow> None | Some dst \<Rightarrow> (
-                  Some (2, Porl_rr dst src) )))
-              else None
-            \<comment> \<open> P2893 `XOR register1 to register2` -> ` 0011 000w : 11 reg1 reg2` \<close>
-            else if h = 0x31 then
-              if modrm = 0b11 then (
-                case ireg_of_u8 src of None \<Rightarrow> None | Some src \<Rightarrow> (
-                case ireg_of_u8 dst of None \<Rightarrow> None | Some dst \<Rightarrow> (
-                  Some (2, Pxorl_rr dst src))) ) 
-              else None
-            else if h = 0xd3 then
-              \<comment> \<open> P2889 `SHL register by CL`              -> ` 1100 000w : 11 100 reg ` \<close>
-              if modrm = 0b11 \<and> reg1 = 0b100 then 
-                case ireg_of_u8 dst of None \<Rightarrow> None | Some dst \<Rightarrow> (
-                  Some (2, Pshll_r dst))
-              \<comment> \<open> P2890 `SHR register by CL`              -> ` 1100 000w : 11 101 reg ` \<close>
-              else if modrm = 0b11 \<and> reg1 = 0b101 then
-                case ireg_of_u8 dst of None \<Rightarrow> None | Some dst \<Rightarrow> (
-                  Some (2, Pshrl_r dst))  
-              \<comment> \<open> P2888 `SAR register by CL`              -> ` 1100 000w : 11 111 reg ` \<close>
-              else if modrm = 0b11 \<and> reg1 = 0b111 then
-                case ireg_of_u8 dst of None \<Rightarrow> None | Some dst \<Rightarrow> (
-                  Some (2, Psarl_r dst))  
-            else None
-            \<comment> \<open> P2892 `TEST: register1 and register2`   -> ` 1000 010w : 11 reg1 reg2` \<close>
-            else if h = 0x85 then
-              if modrm = 0b11 then(
-                case ireg_of_u8 src of None \<Rightarrow> None | Some src \<Rightarrow> (
-                case ireg_of_u8 dst of None \<Rightarrow> None | Some dst \<Rightarrow> (
-                  Some(2, Ptestl_rr dst src) )))
-              else None
-            \<comment> \<open> P2878 `CMP: register1 with register2`   -> ` 0011 100w : 11 reg1 reg2 ` \<close>
-            else if h = 0x39 then
-              if modrm = 0b11 then(
-                case ireg_of_u8 src of None \<Rightarrow> None | Some src \<Rightarrow> (
-                case ireg_of_u8 dst of None \<Rightarrow> None | Some dst \<Rightarrow> (
-                  Some(2, Pcmpl_rr src dst) )))
-              else None
-            else if h = 0xff then
-            \<comment> \<open> P2878 `CALL: register indirect`   -> `0100 W00Bw 1111 1111 : 11 010 reg ` \<close>
-              if modrm = 0b11 \<and> reg1 = 0b010 then
-                case ireg_of_u8 dst of None \<Rightarrow> None | Some dst \<Rightarrow> (
-                  Some (2, Pcall_r dst)) 
-              else None
-            \<comment> \<open> R3 [opcode + modrm + imm] \<close>
-            \<comment> \<open> P2882 `MOV immediate to register` -> ` 1100 011w : 11 000 reg : imm` \<close>
-            else if h = 0xc7 then
-              case nth_error l_bin (pc+2) of None \<Rightarrow> None | Some i1 \<Rightarrow> (
-              case nth_error l_bin (pc+3) of None \<Rightarrow> None | Some i2 \<Rightarrow> (
-              case nth_error l_bin (pc+4) of None \<Rightarrow> None | Some i3 \<Rightarrow> (
-              case nth_error l_bin (pc+5) of None \<Rightarrow> None | Some i4 \<Rightarrow> (
-              case ireg_of_u8 dst of None \<Rightarrow> None | Some dst \<Rightarrow> (
-              case u32_of_u8_list [i1, i2, i3, i4] of None \<Rightarrow> None |
-                  Some imm \<Rightarrow> 
-                    if modrm = 0b11 \<and> reg1 = 0b000 then
-                      Some (6, Pmovl_ri dst imm)
-                    else None) ))))
-            else if h = 0xc1 then
-              case nth_error l_bin (pc+2) of None \<Rightarrow> None | Some imm \<Rightarrow> ( 
-                \<comment> \<open> P2889 `SHL register by immediate count`      -> `1100 000w : 11 100 reg : imm8 ` \<close>
-                if modrm = 0b11 \<and> reg1 = 0b100 then 
-                  case ireg_of_u8 dst of None \<Rightarrow> None | Some dst \<Rightarrow> (
-                     Some (3, Pshll_ri dst imm))
-                \<comment> \<open> P2890 `SHR register by immediate count`      -> ` 1100 000w : 11 101 reg : imm8 ` \<close>
-                else if modrm = 0b11 \<and> reg1 = 0b101 then 
-                  case ireg_of_u8 dst of None \<Rightarrow> None | Some dst \<Rightarrow> (
-                     Some (3, Pshrl_ri dst imm))
-                \<comment> \<open> P2888 `SAR register by immediate count`      -> `1100 000w : 11 111 reg : imm8 ` \<close>
-                else if modrm = 0b11 \<and> reg1 = 0b111 then 
-                  case ireg_of_u8 dst of None \<Rightarrow> None | Some dst \<Rightarrow> (
-                     Some (3, Psarl_ri dst imm))
-                 else None)
-            else if h = 0x81 then
-              if modrm = 0b11 then
-                case ireg_of_u8 dst of None \<Rightarrow> None | Some dst \<Rightarrow> (
-                  case nth_error l_bin (pc+2) of None \<Rightarrow> None | Some i1 \<Rightarrow> (
-                  case nth_error l_bin (pc+3) of None \<Rightarrow> None | Some i2 \<Rightarrow> (
-                  case nth_error l_bin (pc+4) of None \<Rightarrow> None | Some i3 \<Rightarrow> (
-                  case nth_error l_bin (pc+5) of None \<Rightarrow> None | Some i4 \<Rightarrow> (
-                    case u32_of_u8_list [i1,i2,i3,i4] of None \<Rightarrow> None |
-                      Some imm \<Rightarrow> 
-                        \<comment> \<open> P2876 `ADD immediate to register` -> ` 1000 00sw : 11 000 reg : immediate data` \<close>
-                        if reg1 = 0b000 then
-                          Some (6, Paddl_ri dst imm)
-                        \<comment> \<open> P2891 `OR: immediate to register` -> `0100 000B  1000 00sw : 11 001 reg : imm` \<close>
-                        else if reg1 = 0b001 then
-                          Some (6, Porl_ri dst imm)
-                        \<comment> \<open> P2891 `AND: immediate to register` -> `0100 000B : 1000 00sw : 11 100 reg : immediate` \<close>
-                        else if reg1 = 0b100 then
-                          Some (6, Pandl_ri dst imm)
-                        \<comment> \<open> P2891 `SUB: immediate from register` -> `0100 000B 1000 00sw : 11 101 reg : imm` \<close>
-                        else if reg1 = 0b101 then
-                          Some (6, Psubl_ri dst imm)
-                        \<comment> \<open> P2893 `XOR: immediate to register` -> ` 0100 000B 1000 00sw : 11 110 reg : imm` \<close>
-                        else if reg1 = 0b110 then
-                          Some (6, Pxorl_ri dst imm)
-                        \<comment> \<open> P2878 `CMP: immediate32 with qwordregister`   -> `0100 100B 1000 0001 : 11 111 qwordreg : imm32` \<close>
-                        else if reg1 = 0b111 then
-                          Some (6, Pcmpl_ri dst imm)
-                        else None) ))))
-              else None
-            \<comment> \<open> R5 [opcode + modrm + displacement] \<close>
-            \<comment> \<open> P2882 ` MOV: memory to reg`   ->  `0100 0RXB : 1000 101w : mod reg r/m`\<close>
-            else if h = 0x88 then
-              if modrm = 0b01  then
-                case nth_error l_bin (pc+2) of None \<Rightarrow> None | Some dis \<Rightarrow> ( \<comment> \<open> displacement8 \<close>
-                  case ireg_of_u8 src of None \<Rightarrow> None | Some src \<Rightarrow> (
-                  case ireg_of_u8 dst of None \<Rightarrow> None | Some dst \<Rightarrow> ( 
-                    Some (3, Pmov_mr (Addrmode (Some dst) None (scast dis)) src  M8))) )
-              else None
-            else if h = 0x8b then 
-              if modrm = 0b01 then
-                case nth_error l_bin (pc+2) of None \<Rightarrow> None | Some dis \<Rightarrow> ( \<comment> \<open> displacement8 \<close>
-                    case ireg_of_u8 src of None \<Rightarrow> None | Some src \<Rightarrow> (
-                    case ireg_of_u8 dst of None \<Rightarrow> None | Some dst \<Rightarrow> (
-                      Some (3, Pmov_rm src (Addrmode (Some dst) None (scast dis))  M32))) )
-              else if modrm = 0b10 then \<comment> \<open> displacement32 \<close>
-                case nth_error l_bin (pc+2) of None \<Rightarrow> None | Some d1 \<Rightarrow> (
-                case nth_error l_bin (pc+3) of None \<Rightarrow> None | Some d2 \<Rightarrow> (
-                case nth_error l_bin (pc+4) of None \<Rightarrow> None | Some d3 \<Rightarrow> (
-                case nth_error l_bin (pc+5) of None \<Rightarrow> None | Some d4 \<Rightarrow> (
-                  case u32_of_u8_list [d1,d2,d3,d4] of None \<Rightarrow> None | Some dis \<Rightarrow>(
-                  case ireg_of_u8 src of None \<Rightarrow> None | Some src \<Rightarrow> (
-                  case ireg_of_u8 dst of None \<Rightarrow> None | Some dst \<Rightarrow> (
-                     Some (6, Pmov_rm src (Addrmode (Some dst) None dis) M32)))) ))))
-              else None
-            else None
+        x64_decode_op_not_rex h pc l_bin
     else if unsigned_bitfield_extract_u8 0 4 h = 0 then   \<comment> \<open> h is rex, the low 4-bit must not 0  \<close> 
       None
     else  \<comment> \<open> h is rex  \<close> 
@@ -765,27 +852,25 @@ definition x64_decode :: "nat \<Rightarrow> x64_bin \<Rightarrow> (nat * instruc
                 Some (3, Pcall_r dst)
               else None) 
         \<comment> \<open> P2885 `PUSH: memory64`   -> `0100 W00BS : 1111 1111 : mod 110 r/m ` \<close>
-          else if modrm = 0b10 then 
-            if reg2 = 0b100 then                           
-              case nth_error l_bin (pc+3) of None \<Rightarrow> None | Some sib \<Rightarrow> (
-              let rbase  = unsigned_bitfield_extract_u8 0 3 sib in
-              let rindex = unsigned_bitfield_extract_u8 3 3 sib in
-              let scale  = unsigned_bitfield_extract_u8 6 2 sib in
-              let index  = bitfield_insert_u8 3 1 rindex x in
-              let base   = bitfield_insert_u8 3 1 rbase  b in
-                case nth_error l_bin (pc+4) of None \<Rightarrow> None | Some d1 \<Rightarrow> (
-                case nth_error l_bin (pc+5) of None \<Rightarrow> None | Some d2 \<Rightarrow> (
-                case nth_error l_bin (pc+6) of None \<Rightarrow> None | Some d3 \<Rightarrow> (
-                case nth_error l_bin (pc+7) of None \<Rightarrow> None | Some d4 \<Rightarrow> (
-                  case u32_of_u8_list [d1,d2,d3,d4] of None \<Rightarrow> None | Some dis \<Rightarrow>(
-                  if reg1 = 0b110 then
-                    if w = 1 \<and> r = 0 then
-                      case ireg_of_u8 index of None \<Rightarrow> None | Some ri \<Rightarrow> (
-                      case ireg_of_u8 base  of None \<Rightarrow> None | Some rb \<Rightarrow> (
-                        Some (8, Ppushq_m (Addrmode (Some rb) (Some (ri, scale)) (scast dis)) M64 )))
-                    else None
-                  else None) )))) )
-            else None
+          else if modrm = 0b10 \<and> reg2 = 0b100 then                           
+            case nth_error l_bin (pc+3) of None \<Rightarrow> None | Some sib \<Rightarrow> (
+            let rbase  = unsigned_bitfield_extract_u8 0 3 sib in
+            let rindex = unsigned_bitfield_extract_u8 3 3 sib in
+            let scale  = unsigned_bitfield_extract_u8 6 2 sib in
+            let index  = bitfield_insert_u8 3 1 rindex x in
+            let base   = bitfield_insert_u8 3 1 rbase  b in
+              case nth_error l_bin (pc+4) of None \<Rightarrow> None | Some d1 \<Rightarrow> (
+              case nth_error l_bin (pc+5) of None \<Rightarrow> None | Some d2 \<Rightarrow> (
+              case nth_error l_bin (pc+6) of None \<Rightarrow> None | Some d3 \<Rightarrow> (
+              case nth_error l_bin (pc+7) of None \<Rightarrow> None | Some d4 \<Rightarrow> (
+                case u32_of_u8_list [d1,d2,d3,d4] of None \<Rightarrow> None | Some dis \<Rightarrow>(
+                if reg1 = 0b110 then
+                  if w = 1 \<and> r = 0 then
+                    case ireg_of_u8 index of None \<Rightarrow> None | Some ri \<Rightarrow> (
+                    case ireg_of_u8 base  of None \<Rightarrow> None | Some rb \<Rightarrow> (
+                      Some (8, Ppushq_m (Addrmode (Some rb) (Some (ri, scale)) (scast dis)) M64 )))
+                  else None
+                else None) )))) )
           else None
         \<comment> \<open> R6.4 [rex + opcode + modrm + imm] \<close>
         else if op = 0xc7 then
@@ -823,75 +908,7 @@ definition x64_decode :: "nat \<Rightarrow> x64_bin \<Rightarrow> (nat * instruc
                 else None
               else None) ))))
         else if op = 0x81 then
-          if modrm = 0b11 then
-            case ireg_of_u8 dst of None \<Rightarrow> None | Some dst \<Rightarrow> (
-              case nth_error l_bin (pc+3) of None \<Rightarrow> None | Some i1 \<Rightarrow> (
-              case nth_error l_bin (pc+4) of None \<Rightarrow> None | Some i2 \<Rightarrow> (
-              case nth_error l_bin (pc+5) of None \<Rightarrow> None | Some i3 \<Rightarrow> (
-              case nth_error l_bin (pc+6) of None \<Rightarrow> None | Some i4 \<Rightarrow> (
-                case u32_of_u8_list [i1,i2,i3,i4] of None \<Rightarrow> None |
-                  Some imm \<Rightarrow> (
-                    \<comment> \<open> P2876 `ADD immediate to register` -> `0100 000B : 1000 00sw : 11 000 reg : immediate data` \<close>
-                    if reg1 = 0b000 then
-                      if w = 0 \<and> r = 0 \<and> x = 0 then
-                        Some (7, Paddl_ri dst imm)
-                      else None
-                    \<comment> \<open> P2891 `OR: immediate to register` -> `0100 000B  1000 00sw : 11 001 reg : imm` \<close>
-                    else if reg1 = 0b001 then
-                      if w = 0 \<and> r = 0 \<and> x = 0 then
-                        Some (7, Porl_ri dst imm)
-                      else None
-                    \<comment> \<open> P2891 `AND: immediate to register` -> `0100 000B : 1000 00sw : 11 100 reg : immediate` \<close>
-                    else if reg1 = 0b100 then
-                      if w = 0 \<and> r = 0 \<and> x = 0 then
-                        Some (7, Pandl_ri dst imm)
-                      else None
-                    \<comment> \<open> P2891 `SUB: immediate from register` -> `0100 000B 1000 00sw : 11 101 reg : imm` \<close>
-                    else if reg1 = 0b101 then
-                      if w = 0 \<and> r = 0 \<and> x = 0 then
-                        Some (7, Psubl_ri dst imm)
-                      else None
-                    \<comment> \<open> P2893 `XOR: immediate to register` -> ` 0100 000B 1000 00sw : 11 110 reg : imm` \<close>
-                    else if reg1 = 0b110 then
-                      if w = 0 \<and> r = 0 \<and> x = 0 then
-                        Some (7, Pxorl_ri dst imm)
-                      else None
-                    \<comment> \<open> P2878 `CMP: immediate with register`   -> `0100 000B 1000 00sw : 11 111 reg : imm` \<close>
-                    \<comment> \<open> P2878 `CMP: immediate32 with qwordregister`   -> `0100 100B 1000 0001 : 11 111 qwordreg : imm32` \<close>
-                    else if reg1 = 0b111 then
-                      if w = 1 \<and> r = 0 \<and> x = 0 then
-                        Some (7, Pcmpq_ri dst imm)
-                      else if w = 0 \<and> r = 0 \<and> x = 0 then
-                        Some (7, Pcmpl_ri dst imm)
-                      else None
-                    else None)) ))))
-          else if modrm = 0b10 then
-            if reg2 = 0b100 then
-              case nth_error l_bin (pc+3) of None \<Rightarrow> None | Some sib \<Rightarrow> (
-              let rbase  = unsigned_bitfield_extract_u8 0 3 sib in
-              let rindex = unsigned_bitfield_extract_u8 3 3 sib in
-              let scale  = unsigned_bitfield_extract_u8 6 2 sib in
-              let index  = bitfield_insert_u8 3 1 rindex x in
-              let base   = bitfield_insert_u8 3 1 rbase  b in
-                case nth_error l_bin (pc+4) of None \<Rightarrow> None | Some d1 \<Rightarrow> (
-                case nth_error l_bin (pc+5) of None \<Rightarrow> None | Some d2 \<Rightarrow> (
-                case nth_error l_bin (pc+6) of None \<Rightarrow> None | Some d3 \<Rightarrow> (
-                case nth_error l_bin (pc+7) of None \<Rightarrow> None | Some d4 \<Rightarrow> (
-                  case u32_of_u8_list [d1,d2,d3,d4] of None \<Rightarrow> None | Some dis \<Rightarrow>(
-                  if reg1 = 0b000 then
-                    case nth_error l_bin (pc+8) of None \<Rightarrow> None | Some i1 \<Rightarrow> (
-                    case nth_error l_bin (pc+9) of None \<Rightarrow> None | Some i2 \<Rightarrow> (
-                    case nth_error l_bin (pc+10) of None \<Rightarrow> None | Some i3 \<Rightarrow> (
-                    case nth_error l_bin (pc+11) of None \<Rightarrow> None | Some i4 \<Rightarrow> (
-                    case u32_of_u8_list [i1,i2,i3,i4] of None \<Rightarrow> None | Some imm \<Rightarrow> (
-                    if w = 1 \<and> r = 0 then
-                      case ireg_of_u8 index of None \<Rightarrow> None | Some ri \<Rightarrow> (
-                      case ireg_of_u8 base  of None \<Rightarrow> None | Some rb \<Rightarrow> (
-                        Some (12, Paddq_mi (Addrmode (Some rb) (Some (ri, scale)) (scast dis)) imm M64 )))
-                    else None) ))))
-                  else None) )))) )
-            else None
-          else None
+          x64_decode_op_0x81 modrm dst reg1 reg2 w r x b pc l_bin
         else if op = 0xc1 then
           case nth_error l_bin (pc+3) of None \<Rightarrow> None | Some imm \<Rightarrow> (
         \<comment> \<open> P2889 `SHL register by immediate count`      -> ` 0100 000B 1100 000w : 11 100 reg : imm8 ` \<close>
@@ -988,6 +1005,7 @@ definition x64_decode :: "nat \<Rightarrow> x64_bin \<Rightarrow> (nat * instruc
     \<comment> \<open> R6.6 [rex + opcode + modrm + displacement + imm] \<close>
         else None ))
 )"
+
 
 (*
 fun x64_disassemble_aux :: "nat \<Rightarrow> nat \<Rightarrow> x64_bin \<Rightarrow> x64_asm option" where
