theory/x64DecodeProp.thy
@@ -1,0 +1,364 @@
+theory x64DecodeProp
+imports
+  Main
+  rBPFCommType
+  x64Disassembler
+begin
+
+lemma list_in_list_nth_error_0:
+  "list_in_list l0 pc l \<Longrightarrow> nth_error l0 0 = Some v \<Longrightarrow> nth_error l pc = Some v"
+  apply (induction l0 arbitrary: l pc)
+  subgoal for l pc
+    by (simp add: nth_error_def)
+  subgoal for a l0 l pc
+    apply (simp add: nth_error_def)
+    apply (cases "length l \<le> pc"; simp)
+    done
+  done
+
+lemma list_in_list_nth_error:
+  "list_in_list l0 pc l \<Longrightarrow> nth_error l0 n = Some v \<Longrightarrow> nth_error l (pc+n) = Some v"
+  apply (induction n arbitrary: l0 l pc)
+  subgoal for l0 l pc
+    apply simp
+    using list_in_list_nth_error_0 by metis
+  subgoal for n l0 l pc
+    apply (simp add: nth_error_def)
+    apply (cases l0)
+    subgoal by auto
+    subgoal for a tl0
+      apply simp
+      apply (cases "nth_error l pc"; simp)
+      apply (cases "length tl0 \<le> n"; simp)
+      by fastforce
+    done
+  done
+
+lemma list_in_list_x64_decode:
+  "list_in_list l_bin pc l \<Longrightarrow> x64_decode 0 l_bin = Some v \<Longrightarrow> x64_decode pc l = Some v"
+  apply (simp add: x64_decode_def)
+  apply (cases "nth_error l_bin 0"; simp)
+  apply (frule list_in_list_nth_error [of _ _ _ 0 _], assumption, simp)
+  subgoal for h
+    apply (cases "h = 144"; simp)
+    apply (cases "h = 153"; simp)
+    apply (cases "h = 195"; simp)
+    apply (cases "h = 102"; simp)
+     prefer 2
+     apply (cases "h = 15"; simp)
+      prefer 2
+      apply (cases "and 15 (h >> 4) \<noteq> 4"; simp)
+    prefer 2
+      apply (cases "and 15 h = 0"; simp)
+       apply (cases "nth_error l_bin (Suc 0)"; simp)
+      apply (frule list_in_list_nth_error [of _ _ _ "Suc 0" _], assumption, simp)
+    subgoal for op
+      apply (cases "op = 153"; simp)
+      apply (cases "and 31 (op >> 3) = 10"; simp)
+      apply (cases "and 31 (op >> 3) = 11"; simp)
+      apply (cases "and 31 (op >> 3) = 23"; simp)
+
+      subgoal
+        apply (cases "nth_error l_bin (Suc (Suc 0))"; simp)
+          apply (frule list_in_list_nth_error [of _ _ _ "Suc (Suc 0)" _], assumption, simp)
+        subgoal for i1 apply (cases "nth_error l_bin 3"; simp)
+          apply (frule list_in_list_nth_error [of _ _ _ 3 _], assumption, simp)
+        subgoal for i2 apply (cases "nth_error l_bin 4"; simp)
+          apply (frule list_in_list_nth_error [of _ _ _ 4 _], assumption, simp)
+        subgoal for i3 apply (cases "nth_error l_bin 5"; simp)
+          apply (frule list_in_list_nth_error [of _ _ _ 5 _], assumption, simp)
+        subgoal for i4 apply (cases "nth_error l_bin 6"; simp)
+          apply (frule list_in_list_nth_error [of _ _ _ 6 _], assumption, simp)
+        subgoal for i5 apply (cases "nth_error l_bin 7"; simp)
+          apply (frule list_in_list_nth_error [of _ _ _ 7 _], assumption, simp)
+        subgoal for i6 apply (cases "nth_error l_bin 8"; simp)
+          apply (frule list_in_list_nth_error [of _ _ _ 8 _], assumption, simp)
+        subgoal for i7 apply (cases "nth_error l_bin 9"; simp)
+          apply (frule list_in_list_nth_error [of _ _ _ 9 _], assumption, simp)
+          done done done done done done done done
+
+        apply (cases "op = 104"; simp)
+        subgoal
+          apply (cases "nth_error l_bin (Suc (Suc 0))"; simp)
+          apply (frule list_in_list_nth_error [of _ _ _ "Suc (Suc 0)" _], assumption, simp)
+          subgoal for i1 apply (cases "nth_error l_bin 3"; simp)
+          apply (frule list_in_list_nth_error [of _ _ _ 3 _], assumption, simp)
+          subgoal for i2 apply (cases "nth_error l_bin 4"; simp)
+          apply (frule list_in_list_nth_error [of _ _ _ 4 _], assumption, simp)
+          subgoal for i3 apply (cases "nth_error l_bin 5"; simp)
+          apply (frule list_in_list_nth_error [of _ _ _ 5 _], assumption, simp)
+          done done done done 
+
+        apply (cases "op = 15"; simp)
+        subgoal
+          apply (cases "nth_error l_bin (Suc (Suc 0))"; simp)
+          apply (frule list_in_list_nth_error [of _ _ _ "Suc (Suc 0)" _], assumption, simp)
+          subgoal for i1 apply (cases "and 31 (i1 >> 3) = 25"; simp)
+            apply (cases "and 15 (i1 >> 4) = 4"; simp)
+            apply (cases "nth_error l_bin 3"; simp)
+            apply (frule list_in_list_nth_error [of _ _ _ 3 _], assumption, simp)
+            done done
+
+        apply (cases "nth_error l_bin (Suc (Suc 0))"; simp)
+        apply (frule list_in_list_nth_error [of _ _ _ "Suc (Suc 0)" _], assumption, simp)
+        subgoal for reg apply (cases "op = 137"; simp)
+          subgoal apply (simp add: Let_def) 
+            apply (cases "and 3 (reg >> 6) = 3"; simp)
+            apply (cases "and 3 (reg >> 6) = 1"; simp)
+              subgoal
+                apply (cases "nth_error l_bin 3"; simp)
+                by (frule list_in_list_nth_error [of _ _ _ 3 _], assumption, simp)
+
+            apply (cases "and 3 (reg >> 6) = 2"; simp)
+            apply (cases "and 7 reg \<noteq> 4"; simp)
+              subgoal
+                apply (cases "nth_error l_bin 3"; simp)
+                apply (frule list_in_list_nth_error [of _ _ _ 3 _], assumption, simp)
+                subgoal for d1 apply (cases "nth_error l_bin 4"; simp)
+                apply (frule list_in_list_nth_error [of _ _ _ 4 _], assumption, simp)
+                subgoal for d2 apply (cases "nth_error l_bin 5"; simp)
+                apply (frule list_in_list_nth_error [of _ _ _ 5 _], assumption, simp)
+                subgoal for d3 apply (cases "nth_error l_bin 6"; simp)
+                apply (frule list_in_list_nth_error [of _ _ _ 6 _], assumption, simp)
+                subgoal for d4 apply (cases "u32_of_u8_list [d1, d2, d3, d4]"; simp)
+                subgoal for dis apply (cases "ireg_of_u8 (bitfield_insert_u8 3 (Suc 0) (and 7 (reg >> 3)) (and 1 (h >> 2)))"; simp)
+                subgoal for src apply (cases "ireg_of_u8 (bitfield_insert_u8 3 (Suc 0) (and 7 reg) (and 1 h))"; simp)
+                subgoal for rb 
+                  by argo
+                done done done done done done done
+              
+              apply (cases "nth_error l_bin 3"; simp)
+              apply (frule list_in_list_nth_error [of _ _ _ 3 _], assumption, simp)
+              subgoal for d1 apply (cases "nth_error l_bin 4"; simp)
+              apply (frule list_in_list_nth_error [of _ _ _ 4 _], assumption, simp)
+              subgoal for d2 apply (cases "nth_error l_bin 5"; simp)
+              apply (frule list_in_list_nth_error [of _ _ _ 5 _], assumption, simp)
+              subgoal for d3 apply (cases "nth_error l_bin 6"; simp)
+              apply (frule list_in_list_nth_error [of _ _ _ 6 _], assumption, simp)
+              subgoal for d4 apply (cases "nth_error l_bin 7"; simp)
+              apply (frule list_in_list_nth_error [of _ _ _ 7 _], assumption, simp)
+              done done done done done
+
+            apply (cases "op = 135"; simp)
+            subgoal 
+              apply (simp add: Let_def)
+              apply (cases "and 3 (reg >> 6) = 3"; simp)
+              apply (cases "and 3 (reg >> 6) = 2"; simp)
+              apply (cases " and 7 reg = 4"; simp)
+              apply (cases "nth_error l_bin 3"; simp)
+              apply (frule list_in_list_nth_error [of _ _ _ 3 _], assumption, simp)
+              subgoal for d1 apply (cases "nth_error l_bin 4"; simp)
+              apply (frule list_in_list_nth_error [of _ _ _ 4 _], assumption, simp)
+              subgoal for d2 apply (cases "nth_error l_bin 5"; simp)
+              apply (frule list_in_list_nth_error [of _ _ _ 5 _], assumption, simp)
+              subgoal for d3 apply (cases "nth_error l_bin 6"; simp)
+              apply (frule list_in_list_nth_error [of _ _ _ 6 _], assumption, simp)
+              subgoal for d4 apply (cases "nth_error l_bin 7"; simp)
+              apply (frule list_in_list_nth_error [of _ _ _ 7 _], assumption, simp)
+              done done done done done
+
+            apply (cases "op = 99"; simp)
+            apply (cases "op = 1"; simp)
+            apply (cases "op = 41"; simp)
+            apply (cases "op = 247"; simp)
+            subgoal
+              apply (simp add: Let_def)
+
+              apply (cases "and 3 (reg >> 6) = 3 \<and> and 7 (reg >> 3) = 3"; simp)
+              apply (cases "and 3 (reg >> 6) = 3 \<and> and 7 (reg >> 3) = 4"; simp)
+              apply (cases "and 3 (reg >> 6) = 3 \<and> and 7 (reg >> 3) = 5"; simp)
+              apply (cases "and 3 (reg >> 6) = 3 \<and> and 7 (reg >> 3) = 6"; simp)
+              apply (cases "and 3 (reg >> 6) = 3 \<and> and 7 (reg >> 3) = 7"; simp)
+              apply (cases "and 3 (reg >> 6) = 3 \<and> and 7 (reg >> 3) = 0"; simp)
+              apply (cases "nth_error l_bin 3"; simp)
+              apply (frule list_in_list_nth_error [of _ _ _ 3 _], assumption, simp)
+              subgoal for d1 apply (cases "nth_error l_bin 4"; simp)
+              apply (frule list_in_list_nth_error [of _ _ _ 4 _], assumption, simp)
+              subgoal for d2 apply (cases "nth_error l_bin 5"; simp)
+              apply (frule list_in_list_nth_error [of _ _ _ 5 _], assumption, simp)
+              subgoal for d3 apply (cases "nth_error l_bin 6"; simp)
+              apply (frule list_in_list_nth_error [of _ _ _ 6 _], assumption, simp)
+              done done done done
+
+            apply (cases "op = 9"; simp)
+            apply (cases "op = 33"; simp)
+            apply (cases "op = 49"; simp)
+            apply (cases "op = 211"; simp)
+            apply (cases "op = 133"; simp)
+            apply (cases "op = 57"; simp)
+            apply (cases "op = 255"; simp)
+            subgoal
+              apply (simp add: Let_def)
+
+              apply (cases "and 3 (reg >> 6) = 3 \<and> and 7 (reg >> 3) = 2"; simp)
+              apply (cases "and 3 (reg >> 6) = 2 \<and> and 7 reg = 4"; simp)
+              apply (cases "nth_error l_bin 3"; simp)
+              apply (frule list_in_list_nth_error [of _ _ _ 3 _], assumption, simp)
+              subgoal for sib apply (cases "nth_error l_bin 4"; simp)
+              apply (frule list_in_list_nth_error [of _ _ _ 4 _], assumption, simp)
+              subgoal for d1 apply (cases "nth_error l_bin 5"; simp)
+              apply (frule list_in_list_nth_error [of _ _ _ 5 _], assumption, simp)
+              subgoal for d2 apply (cases "nth_error l_bin 6"; simp)
+              apply (frule list_in_list_nth_error [of _ _ _ 6 _], assumption, simp)
+              subgoal for d3 apply (cases "nth_error l_bin 7"; simp)
+              apply (frule list_in_list_nth_error [of _ _ _ 7 _], assumption, simp)
+              done done done done done
+
+            apply (cases "op = 199"; simp)
+            subgoal
+              apply (simp only: Let_def)
+
+              apply (cases "and 3 (reg >> 6) = 1"; simp)
+              subgoal apply (cases "nth_error l_bin 4"; simp)
+                subgoal for i1 apply (frule list_in_list_nth_error [of _ _ _ 4 i1]) apply blast
+                  apply (rule subst [of "pc+4" "4+pc"]; simp)
+
+                  apply (cases "nth_error l_bin 5"; simp)
+                  subgoal for i2 apply (frule list_in_list_nth_error [of _ _ _ 5 i2]) apply blast
+                  apply (rule subst [of "pc+5" "5+pc"]; simp)
+
+                  apply (cases "nth_error l_bin 6"; simp)
+                  subgoal for i3 apply (frule list_in_list_nth_error [of _ _ _ 6 i3]) apply blast
+                  apply (rule subst [of "pc+6" "6+pc"]; simp)
+
+                  apply (cases "nth_error l_bin 7"; simp)
+                  subgoal for i4 apply (frule list_in_list_nth_error [of _ _ _ 7 i4]) apply blast
+                  apply (rule subst [of "pc+7" "7+pc"]; simp)
+                  apply (cases "ireg_of_u8 (bitfield_insert_u8 3 (Suc 0) (and 7 reg) (and 1 h))"; simp)
+                  subgoal for dst apply (cases "u32_of_u8_list [i1, i2, i3, i4]"; simp)
+                  subgoal for imm apply (cases "and 7 (reg >> 3) = 0 \<and> and 1 (h >> 2) = 0 \<and> and 1 (h >> Suc 0) = 0"; simp)
+                    apply (cases "and 1 (h >> 3) = 1"; simp)
+                    apply (cases "nth_error l_bin 3"; simp)
+                    apply (frule list_in_list_nth_error [of _ _ _ 3 _], assumption, simp)
+                    done done done done done done done
+
+                  apply (cases "and 3 (reg >> 6) = 2"; simp)
+                  subgoal
+                    apply (cases "nth_error l_bin 7"; simp)
+                    apply (frule list_in_list_nth_error [of _ _ _ 7 _], assumption)
+                    apply (rule subst [of "pc+7" "7+pc"]; simp)
+
+                    subgoal for i1
+                      apply (cases "nth_error l_bin 8"; simp)
+                      subgoal for i2 apply (frule list_in_list_nth_error [of _ _ _ 8 i2]) apply blast
+                        apply (rule subst [of "pc+8" "8+pc"]; simp)
+
+                      apply (cases "nth_error l_bin 9"; simp)
+                      subgoal for i3 apply (frule list_in_list_nth_error [of _ _ _ 9 i3]) apply blast
+                        apply (rule subst [of "pc+9" "9+pc"]; simp)
+
+                      apply (cases "nth_error l_bin 10"; simp)
+                      subgoal for i4 apply (frule list_in_list_nth_error [of _ _ _ 10 i4]) apply blast
+                        apply (rule subst [of "pc+10" "10+pc"]; simp)
+
+                        apply (cases "ireg_of_u8 (bitfield_insert_u8 3 (Suc 0) (and 7 reg) (and 1 h))"; simp)
+                        subgoal for dst apply (cases "u32_of_u8_list [i1, i2, i3, i4]"; simp)
+                          apply (cases "and 7 (reg >> 3) = 0 \<and> and 1 (h >> 2) = 0 \<and> and 1 (h >> Suc 0) = 0"; simp)
+
+                          apply (cases "nth_error l_bin 3"; simp)
+                          apply (frule list_in_list_nth_error [of _ _ _ 3 _], assumption, simp)
+                          subgoal for sib apply (cases "nth_error l_bin 4"; simp)
+                          apply (frule list_in_list_nth_error [of _ _ _ 4 _], assumption, simp)
+                          subgoal for d1 apply (cases "nth_error l_bin 5"; simp)
+                          apply (frule list_in_list_nth_error [of _ _ _ 5 _], assumption, simp)
+                          subgoal for d2 apply (cases "nth_error l_bin 6"; simp)
+                          apply (frule list_in_list_nth_error [of _ _ _ 6 _], assumption, simp)
+                            done done done done done done done done done
+
+                  apply (cases "nth_error l_bin 3"; simp)
+                  apply (frule list_in_list_nth_error [of _ _ _ 3 _], assumption, simp)
+                  subgoal for i1 apply (cases "nth_error l_bin 4"; simp)
+                  apply (frule list_in_list_nth_error [of _ _ _ 4 _], assumption, simp)
+                  subgoal for i2 apply (cases "nth_error l_bin 5"; simp)
+                  apply (frule list_in_list_nth_error [of _ _ _ 5 _], assumption, simp)
+                  subgoal for i3 apply (cases "nth_error l_bin 6"; simp)
+                  apply (frule list_in_list_nth_error [of _ _ _ 6 _], assumption, simp)
+                  subgoal for i4 apply (cases "ireg_of_u8 (bitfield_insert_u8 3 (Suc 0) (and 7 reg) (and 1 h))"; simp)
+                  subgoal for dst apply (cases "u32_of_u8_list [i1, i2, i3, i4]"; simp)
+                  subgoal for imm apply (cases "and 7 (reg >> 3) = 0 \<and> and 1 (h >> 2) = 0 \<and> and 1 (h >> Suc 0) = 0"; simp)
+                  apply (cases "and 3 (reg >> 6) = 3"; simp)
+                  apply (cases "and 1 (h >> 3) = 0"; simp)
+                    done done done done done done done
+
+                  apply (cases "op = 129"; simp)
+                  subgoal 
+                    apply (simp add: Let_def)
+                    sorry
+
+                  apply (cases "op = 193"; simp)
+                  subgoal
+                    apply (cases "nth_error l_bin 3"; simp)
+                    apply (frule list_in_list_nth_error [of _ _ _ 3 _], assumption, simp)
+                    done
+
+                  apply (cases "op = 136"; simp)
+                  subgoal
+                    apply (cases "and 3 (reg >> 6) = 1 \<and> and 1 (h >> Suc 0) = 0 \<and> and 1 (h >> 3) = 0"; simp)
+                    apply (cases "nth_error l_bin 3"; simp)
+                    apply (frule list_in_list_nth_error [of _ _ _ 3 _], assumption, simp)
+                    done
+
+                  apply (cases "op = 139"; simp)
+                  subgoal
+                    apply (simp add: Let_def)
+                    apply (cases "and 3 (reg >> 6) = 1 \<and> and 1 (h >> Suc 0) = 0"; simp)
+                    apply (cases "nth_error l_bin 3"; simp)
+                    apply (frule list_in_list_nth_error [of _ _ _ 3 _], assumption, simp)
+                    subgoal for dis apply (cases "ireg_of_u8 (bitfield_insert_u8 3 (Suc 0) (and 7 (reg >> 3)) (and 1 (h >> 2)))"; simp)
+                    subgoal for src apply (cases "ireg_of_u8 (bitfield_insert_u8 3 (Suc 0) (and 7 reg) (and 1 h))"; simp)
+                    subgoal for dst by force 
+                    done done
+
+                  apply (cases "and 3 (reg >> 6) = 2"; simp)
+                  apply (cases "and 7 reg \<noteq> 4"; simp)
+                  subgoal
+                    apply (cases "nth_error l_bin 3"; simp)
+                    apply (frule list_in_list_nth_error [of _ _ _ 3 _], assumption, simp)
+                    apply (cases "nth_error l_bin 4"; simp)
+                    apply (frule list_in_list_nth_error [of _ _ _ 4 _], assumption, simp)
+                    apply (cases "nth_error l_bin 5"; simp)
+                    apply (frule list_in_list_nth_error [of _ _ _ 5 _], assumption, simp)
+                    apply (cases "nth_error l_bin 6"; simp)
+                    apply (frule list_in_list_nth_error [of _ _ _ 6 _], assumption, simp)
+                    subgoal for d1 d2 d3 d4 apply (cases "u32_of_u8_list [d1, d2, d3, d4]"; simp)
+                    subgoal for dis apply (cases "ireg_of_u8 (bitfield_insert_u8 3 (Suc 0) (and 7 (reg >> 3)) (and 1 (h >> 2)))"; simp)
+                    subgoal for src apply (cases "ireg_of_u8 (bitfield_insert_u8 3 (Suc 0) (and 7 reg) (and 1 h))"; simp)
+                    subgoal for dst apply (cases "and 1 (h >> Suc 0) = 0"; simp)
+                      by argo
+                    done done done done
+
+                  apply (cases "nth_error l_bin 3"; simp)
+                  apply (frule list_in_list_nth_error [of _ _ _ 3 _], assumption, simp)
+                  apply (cases "nth_error l_bin 4"; simp)
+                  apply (frule list_in_list_nth_error [of _ _ _ 4 _], assumption, simp)
+                  apply (cases "nth_error l_bin 5"; simp)
+                  apply (frule list_in_list_nth_error [of _ _ _ 5 _], assumption, simp)
+                  apply (cases "nth_error l_bin 6"; simp)
+                  apply (frule list_in_list_nth_error [of _ _ _ 6 _], assumption, simp)
+                  apply (cases "nth_error l_bin 7"; simp)
+                  apply (frule list_in_list_nth_error [of _ _ _ 7 _], assumption, simp)
+                  done
+
+                apply (cases "op = 141"; simp)
+                subgoal
+                  apply (simp add: Let_def)
+                  apply (cases "and 3 (reg >> 6) = 1"; simp)
+                  subgoal
+                    apply (cases "nth_error l_bin 3"; simp)
+                    apply (frule list_in_list_nth_error [of _ _ _ 3 _], assumption, simp)
+                    done
+                  apply (cases "and 3 (reg >> 6) = 2"; simp)
+                  subgoal
+                    apply (cases "nth_error l_bin 3"; simp)
+                    apply (frule list_in_list_nth_error [of _ _ _ 3 _], assumption, simp)
+                    apply (cases "nth_error l_bin 4"; simp)
+                    apply (frule list_in_list_nth_error [of _ _ _ 4 _], assumption, simp)
+                    apply (cases "nth_error l_bin 5"; simp)
+                    apply (frule list_in_list_nth_error [of _ _ _ 5 _], assumption, simp)
+                    apply (cases "nth_error l_bin 6"; simp)
+                    apply (frule list_in_list_nth_error [of _ _ _ 6 _], assumption, simp)
+                    done done done done
+
+                  done
+
+end
